***NO_CI*** adding the update/sel lemmas for IntStoreFixed

examples/dm4free/FStar.DM4F.Heap.IntStoreFixed.fst
@@ -14,3 +14,15 @@ let sel = index
 let upd (h:heap) (i:id) (x:int) : Tot heap = let h1 = upd h i x in assert (length h1 = store_size) ; h1
 
 let create (x:int) : Tot heap = create #int store_size x
+
+abstract val lemma_index_upd1: s:heap -> n:id -> v:int -> Lemma
+  (requires True)
+  (ensures (index (upd s n v) n == v))
+  [SMTPat (index (upd s n v) n)]
+let lemma_index_upd1 s n v = lemma_index_upd1 #int s n v
+
+abstract val lemma_index_upd2: s:heap -> n:id -> v:int -> i:id{i<>n} -> Lemma
+  (requires True)
+  (ensures (index (upd s n v) i == index s i))
+  [SMTPat (index (upd s n v) i)]
+let lemma_index_upd2 s n v i = lemma_index_upd2 #int s n v i
