examples/rel/simple_ifc_reify.fst
@@ -2,28 +2,26 @@ module Simple_Ifc_Reify
 
 open FStar.DM4F.Heap.IntStoreFixed
 open FStar.DM4F.IntStoreFixed
-open FStar.DM4F.ST
 open Rel
 
-let sel=index
 
 (* A very simple program and with different simple properties that can or
 cannot be shown *)
 
 (*****************************************************************************)
 
-reifiable val ifc_a : x:id -> 
-  IntStore unit 
-  (requires (fun _ -> True)) 
+reifiable val ifc_a : x:id ->
+  IntStore unit
+  (requires (fun _ -> True))
   (ensures (fun h0 _ h1 -> h1 = upd h0 x 0))
 reifiable let ifc_a x = write x 0
 (* works *)
 
 (*****************************************************************************)
 
-reifiable val ifc_b : x:id -> 
-  IntStore unit 
-  (requires (fun _ -> True)) 
+reifiable val ifc_b : x:id ->
+  IntStore unit
+  (requires (fun _ -> True))
   (ensures (fun h0 _ h1 -> sel h1 x = 0))
 reifiable let ifc_b x = write x 0
 (* does not work *)
@@ -33,31 +31,31 @@ reifiable let ifc_b x = write x 0
 
 reifiable let ifc_c x = write x 0
 
-let ifc_c_r h x =  normalize_term (snd (reify (ifc_c x) h))
+let ifc_c_r h x =  (* normalize_term *) (snd (reify (ifc_c x) h))
 
 val ni_ifc_c1 : (x:id) -> (h:rel heap) ->
-  Lemma 
+  Lemma
   (requires (R?.l h == R?.r h))
   (ensures  ((ifc_c_r (R?.l h) x) == (ifc_c_r (R?.r h) x)))
 let ni_ifc_c1 x h = ()
 (* works *)
 
 val ni_ifc_c2 : (x:id) -> (h:rel heap) ->
-  Lemma 
+  Lemma
   (requires (R?.l h == R?.r h))
   (ensures  (sel (ifc_c_r (R?.l h) x) x = sel (ifc_c_r (R?.r h) x) x))
 let ni_ifc_c2 x h = ()
 (* works *)
 
 val ni_ifc_c3 : (x:id) -> (h:rel heap) ->
-  Lemma 
+  Lemma
   (requires (sel (R?.l h) x = sel (R?.r h) x))
   (ensures  (sel (ifc_c_r (R?.l h) x) x = sel (ifc_c_r (R?.r h) x) x))
 let ni_ifc_c3 x h = ()
 (* does not work *)
 
 val ni_ifc_c4 : (x:id) -> (h:heap) ->
-  Lemma 
+  Lemma
   (requires True)
   (ensures  (sel (ifc_c_r h x) x = 0))
 let ni_ifc_c4 x h = ()
